add ulibs

src/fstarHelper.c
@@ -1,8 +1,0 @@
-#include <stdio.h>
-
-#include "Main.h"
-
-// debug
-void Main_print_hex(uint8_t i) {
-  printf("%02x", i);
-}
