src/utils.c
@@ -1,0 +1,6 @@
+#include <stdio.h>
+#include "Utils.h"
+
+void Utils_print_hex(uint8_t i) {
+  printf("%02x", i);
+}
