src/main.fst
@@ -4,6 +4,7 @@ module B = LowStar.Buffer
 module M = LowStar.Modifies
 module HS = FStar.HyperStack
 module ST = FStar.HyperStack.ST
+module UT = Utils
 
 open FStar.HyperStack.ST
 open LowStar.BufferOps
@@ -174,10 +175,21 @@ type type_error_message_restrict =
     }
   )
 
-// debug tool
-assume val print_hex (i:U8.t): Stack unit
-  (requires (fun h -> true))
-  (ensures (fun h0 ret h1 -> true))
+let new_line () = print_string "\n"
+
+val buffer_loop: src:B.buffer U8.t -> len:U32.t -> Stack unit
+  (requires fun h0 -> B.live h0 src /\ B.length src = U32.v len )
+  (ensures fun _ _ _ -> true)
+let buffer_loop src len =
+  let inv h (i: nat) = B.live h src in
+  let body (i: U32.t{ 0 <= U32.v i /\ U32.v i < U32.v len }): Stack unit
+    (requires (fun h -> inv h (U32.v i)))
+    (ensures (fun _ _ _ -> true))
+  =
+    let v : U8.t = src.(i) in
+      UT.print_hex v; new_line ()
+  in
+  C.Loops.for 0ul len inv body
 
 val slice_byte:
   byte:U8.t
